Add another proof

example.go
@@ -3,3 +3,8 @@ package ver_example
 func Swap(x, y *int) {
 	*x, *y = *y, *x
 }
+
+func UseSwap(x *int) {
+	var z int
+	Swap(x, &z)
+}
